\subsection{Integrale aus Vorlesung \texorpdfstring{\hfill S.72-74 + S.65}{S.72-74 + S.65}}
\vskip3pt
\small{
$ 
\int x(ax+b)^n dx = \frac{(ax + b)^{n+2}}{(n+2)a^2} - \frac{b(ax + b)^{n+1}}{(n+1)a^2} \\[6pt]
\int \frac{x}{(ax+b)^n} dx  = - \frac{1}{(n-2)a^2 (ax+b)^{n-2}} + \frac{b}{(n-1)a^2 (ax + b)^{n-1}} \\[6pt]
\int x^2 (ax+ b)^n dx = \frac{(ax+b)^{n+3}}{(n+3)a^3} - \frac{2b(ax+b)^{n+2}}{(n+2)a^3} + \frac{b^2 (ax+b)^{n-1}}{(n+1)a^3} \\[6pt]
\int \frac{x}{ax^2 + b} dx = \frac{1}{2a} ln|ax^2 + b| \\[6pt]
\int \frac{x}{(a^2 + x^2)^n} dx = \frac{-1}{2(n-1)(a^2 + x^2)^{n-1}} \\[6pt]
\int \frac{x}{(a^2 - x^2)^n} dx = \frac{1}{2(n-1)(a^2 - x^2)^{n-1}} \\[6pt]
\int \frac{x}{x^4 + 3} dx = \frac{\sqrt{3}}{6} arctan(\frac{x^2}{\sqrt{3}}) \\[6pt]
\int \frac{x}{\sqrt{x^2 + 1}} dx = \sqrt{x^2 + 1} \\[6pt]
\int \frac{x}{x^2 + y^2} dy = arctan(\frac{y}{x}) \\[6pt]
\int \frac{-y}{x^2 + y^2} dx = arctan(\frac{y}{x})  \\[6pt]
\int \frac{x^2 - y^2}{x^2 + y^2} dx = \frac{y}{x^2 + y^2}  \\[6pt]
\int \frac{1}{x^2 + a^2} dx = \frac{1}{a} arctan(\frac{x}{a}) \hskip3pt a \neq 0  \\[6pt] 
\int \frac{1}{x^2 - a^2} dx = \frac{1}{2a} ln(\frac{x-a}{x+a}) \\ [6pt]
\int \frac{1}{x^2 + x} dx = ln(x) - ln(x+1) \\[6pt]
\int \frac{1}{1+x^2} dx = arctan(x) \\[6pt]
\int_{-\infty}^{\infty} \frac{1}{1 + x^2} dx = \pi \\[6pt]
\int \frac{1}{1-x^2} dx = artanh(x) = ln(\sqrt{\frac{1+x}{1-x}}) |x| < 1 \\[6pt]
\int \frac{1}{ax^2 + bx + c} dx = \frac{2arctan(\frac{2ax+b}{\sqrt{4ac - b^2}})}{\sqrt{4ac-b^2}} \\[6pt]
\int \frac{1}{(x^2 + x -6 )} dx = \frac{1}{5} ln \left( \frac{x-2}{x+3} \right) \\[6pt]
\int \frac{1}{x^2 + x + 1} dx = \frac{2}{\sqrt{3}} arctan \left( \frac{2x+1}{\sqrt{3}} \right) \\[6pt]
\int \frac{1}{\sqrt{x^2 + 1}} dx = arsinh(x) = ln(x + \sqrt{x^2 + 1}) \\[6pt]
\int \frac{1}{\sqrt{x^2 - 1}} dx = arcosh(x) = ln(x + \sqrt{x^2 -1}) \hskip3pt 1 \leqslant x \\[6pt]
\int \frac{1}{\sqrt{1-x^2}} dx = arcsin(x) = -arccos(x) \\[6pt]
\int \sqrt{1+x^2} dx = \frac{1}{2} \left( arsinh(x) + x \cdot \sqrt{1+x^2} \right) \\[6pt]
\int \sqrt{1-x^2} dx = \frac{1}{2} \left( arcsin(x) + x \cdot \sqrt{1-x^2} \right) \\[6pt]
\int x^2 \cdot sin(x) dx = -x^2cos(x) + 2sin(x) - 2 cos(x) \\ [6pt]
\int x \cdot sin(ax) dx = \frac{1}{a^2} sin(ax) - \frac{x}{a} cos(ax) \\[6pt]
\int \frac{x}{sin^2(x)} dx = -x \cdot cot(x) + ln(sin(x)) \\ [6pt]
\int \frac{1}{sin^2(x)} dx = -cot(x) = tan(x + \frac{\pi}{2}) \\[6pt]
\int \frac{1}{cos^2(x)} dx = tan(x) \\[6pt]
\int sin^2(x) dx = \frac{1}{2} \left( x - sin(x)cos(x) \right)) \\[6pt]
\int sin^3(x) dx = \frac{1}{12} (cos(3x) - 9 cos(x)) \\[6pt]
\int sin^4(x) dx = \frac{1}{32} (12x - 8sin(2x) + sin(4x)) \\[6pt]
\int cos^2(x) dx = \frac{1}{2} (x + sin(x)cos(x)) \\[6pt]
\int cos^3(x) dx = sin(x) - \frac{sin^3(x)}{3} = \frac{1}{12}(9sin(x) + sin(3x)) \\[6pt]
\int cos^4(x) dx = \frac{1}{32}(12x + 8sin(2x) + sin(4x)) \\[6pt]
\int sin^{3/2}(2x) dx = -\frac{1}{2} cos(2x) \\[6pt]
\int cos^{3/2}(2x) dx = sin(x)cos(x) \\[6pt]
\int cos(2x)dx = \frac{1}{2} sin(2x) \\[6pt]
\int sin(x)cos(x) dx = -\frac{1}{2} cos^2(x) \\[6pt]
\int sin^2(x) cos(x) dx = \frac{1}{3}sin^3(x) \\[6pt]
\int sin(x)cos^n(x) dx = - \frac{1}{n+1} cos^{n+1}(x) \hspace{3pt} n \geqslant 0\\[6pt]
$
}